{
 "cells": [
  {
   "cell_type": "markdown",
   "id": "8474241b",
   "metadata": {},
   "source": [
    "# Question 1"
   ]
  },
  {
   "cell_type": "markdown",
   "id": "a22ef7a5",
   "metadata": {},
   "source": [
    "For each of these functions, write down each of their partial derivitives"
   ]
  },
  {
   "cell_type": "markdown",
   "id": "3190d284",
   "metadata": {},
   "source": [
    "a) $$ f(x,y) = x^2+3xy−y^2 $$"
   ]
  },
  {
   "cell_type": "markdown",
   "id": "f5f7989c",
   "metadata": {},
   "source": [
    "$$\\frac{\\delta f(x, y)}{\\delta x} = 2x + 3y$$\n",
    "$$\\frac{\\delta f(x, y)}{\\delta y} = 3x - 2y$$"
   ]
  },
  {
   "cell_type": "markdown",
   "id": "0404c574",
   "metadata": {},
   "source": [
    "b) $$ f(x,y) = cos(xy) $$"
   ]
  },
  {
   "cell_type": "markdown",
   "id": "f17d0437",
   "metadata": {},
   "source": [
    "$$\\frac{\\delta f(x, y)}{\\delta x} = \\frac{\\delta cos(xy)}{\\delta xy} \\cdot \\frac{\\delta xy}{\\delta x} = -sin(x, y) \\cdot y$$\n",
    "\n",
    "$$\\frac{\\delta f(x, y)}{\\delta y} = \\frac{\\delta cos(xy)}{\\delta xy} \\cdot \\frac{\\delta xy}{\\delta y} = -sin(x, y) \\cdot x$$"
   ]
  },
  {
   "cell_type": "markdown",
   "id": "2287eb4a",
   "metadata": {},
   "source": [
    "c) $$ f(x,y) = (1-x)^2 + 5*(y - x^2)^2 $$"
   ]
  },
  {
   "cell_type": "markdown",
   "id": "3da93165",
   "metadata": {},
   "source": [
    "$$ \\frac{\\delta f(x, y)}{\\delta x} \n",
    "= \\frac{\\delta ( (1 - x)^2 + 5 * (y - x^2)^2 )}{\\delta x} \n",
    "= \\frac{\\delta (1 - x)^2}{\\delta x} + \\frac{\\delta 5 * (y - x^2)^2}{\\delta x} $$\n",
    "$$ = \\frac{\\delta (1 - x)^2}{\\delta (1 - x)} \\cdot \\frac{\\delta (1 - x)}{\\delta x} + \\frac{\\delta 5 * (y - x^2)^2}{\\delta (y - x^2)^2} \\cdot \\frac{\\delta (y - x^2)^2}{\\delta (y - x^2)} \\cdot \\frac{\\delta (y - x^2)}{\\delta x} $$\n",
    "$$ = -2(1 - x) + 5 \\cdot 2 \\cdot (y - x^2) \\cdot (-2x) = -2 + 2x -20xy + 20x^3 $$\n",
    "\n",
    "$$ \\frac{\\delta f(x, y)}{\\delta y} = \\frac{\\delta ( (1 - x)^2 + 5 * (y - x^2)^2 )}{\\delta y} = \\frac{\\delta (1 - x)^2}{\\delta y} + \\frac{\\delta 5 \\cdot (y - x^2)^2}{\\delta y} $$\n",
    "$$ = 0 + 5 \\cdot \\frac{\\delta (y - x^2)^2}{\\delta (y - x^2)} \\cdot \\frac{\\delta (y - x^2)}{\\delta y} = 10 \\cdot (y - x^2) $$"
   ]
  },
  {
   "cell_type": "markdown",
   "id": "8b0cedfc",
   "metadata": {},
   "source": [
    "d) $$ f(x,y) = x^2 + y^2 + x*sin(y) $$"
   ]
  },
  {
   "cell_type": "markdown",
   "id": "de013b77",
   "metadata": {},
   "source": [
    "$$ \\frac{\\delta f(x, y)}{\\delta x} = \\frac{\\delta(x^2 + y^2 + x \\cdot sin(y))}{\\delta x} = \\frac{\\delta x^2}{\\delta x} + \\frac{\\delta y^2}{\\delta x} + \\frac{\\delta x \\cdot sin(y)}{\\delta x} = 2x + sin(y) $$\n",
    "\n",
    "$$ \\frac{\\delta f(x, y)}{\\delta y} = \\frac{\\delta(x^2 + y^2 + x \\cdot sin(y))}{\\delta y} = \\frac{\\delta x^2}{\\delta y} + \\frac{\\delta y^2}{\\delta y} + \\frac{\\delta x \\cdot sin(y)}{\\delta y} = 2y + x cos(y) $$"
   ]
  },
  {
   "cell_type": "markdown",
   "id": "4a2e69df",
   "metadata": {},
   "source": [
    "# Question 2\n",
    "Find the gradient vector of $$f(x, y, z) = zxy - x + \\ln(y)$$\n",
    "\n",
    "Find the gradient vector of \n",
    "$$f(x, y) = \\cos^2(y) - \\sin^2(x)$$\n"
   ]
  },
  {
   "cell_type": "markdown",
   "id": "1ed51041",
   "metadata": {},
   "source": [
    "$$ \\nabla f = (\\frac{\\delta f}{\\delta x}, \\frac{\\delta f}{\\delta y},\\frac{\\delta f}{\\delta z}) = (\\frac{\\delta (zxy - x + lny)}{\\delta x}, \\frac{\\delta (zxy - x + lny)}{\\delta y}, \\frac{\\delta (zxy - x + lny)}{\\delta z})$$\n",
    "$$ = (\\frac{\\delta zxy}{\\delta x} - \\frac{\\delta x}{\\delta x} + \\frac{\\delta lny}{\\delta x}, \\frac{\\delta zxy}{\\delta y} - \\frac{\\delta x}{\\delta y} + \\frac{\\delta lny}{\\delta y}, \\frac{\\delta zxy}{\\delta z} - \\frac{\\delta x}{\\delta z} + \\frac{\\delta lny}{\\delta z}) $$\n",
    "$$ = (xy - 1, zx + \\frac{1}{y}, xy) $$\n",
    "\n",
    "<br>\n",
    "\n",
    "$$ \\nabla f = (\\frac{\\delta f}{\\delta x}, \\frac{\\delta f}{\\delta y}) = (\\frac{\\delta (cos^2y - sin^2x)}{\\delta x}, \\frac{\\delta (cos^2y - sin^2x)}{\\delta y}) $$\n",
    "$$ = (\\frac{\\delta cos^2y}{\\delta x} - \\frac{\\delta sin^2x}{\\delta x}, \\frac{\\delta cos^2y}{\\delta y} - \\frac{\\delta sin^2x}{\\delta y}) $$\n",
    "$$ = (0 - \\frac{\\delta sin^2x}{\\delta sinx} \\cdot \\frac{\\delta sinx}{\\delta x}, \\frac{\\delta cos^2y}{\\delta cosy} \\cdot \\frac{\\delta cosy}{\\delta y} - 0) $$\n",
    "$$ = (-2sinxcosx, -2cosxsinx) = (-2sinxcosx, -2sinxcosx)$$"
   ]
  },
  {
   "cell_type": "markdown",
   "id": "de762c89",
   "metadata": {},
   "source": [
    "# Question 3\n",
    "\n",
    "Find the gradient vector of \n",
    "$f(x, y) = \\ln(x) + y^2 \\text{ at } \n",
    "(1, 3)$\n",
    "\n",
    "\n",
    "Find the gradient vector of \n",
    "$f(x, y, z) = -x + 3xy + 5xyz \\text{ at } \n",
    "(-1, 2, 1)$\n"
   ]
  },
  {
   "cell_type": "markdown",
   "id": "6f470c41",
   "metadata": {},
   "source": [
    "$$ \\nabla f = (\\frac{\\delta f}{\\delta x}, \\frac{\\delta f}{\\delta y}) = (\\frac{\\delta(lnx + y^2)}{\\delta x}, \\frac{\\delta(lnx + y^2)}{\\delta y}) = (\\frac{\\delta lnx}{\\delta x} + \\frac{\\delta y^2}{\\delta x}, \\frac{\\delta lnx}{\\delta y} + \\frac{\\delta y^2}{\\delta y}) = (\\frac{1}{x}, 2y) $$\n",
    "$$ \\text{Now } \\nabla f(1, 3) = (\\frac{1}{1}, 2 \\cdot 3) = (1, 6) $$\n",
    "\n",
    "<br>\n",
    "\n",
    "$$ \\nabla f = (\\frac{\\delta f}{\\delta x}, \\frac{\\delta f}{\\delta y}, \\frac{\\delta f}{\\delta z}) = (\\frac{\\delta (-x + 3xy + 5xyz)}{\\delta x}, \\frac{\\delta (-x + 3xy + 5xyz)}{\\delta y},\\frac{\\delta (-x + 3xy + 5xyz)}{\\delta z}) $$\n",
    "$$ = (\\frac{\\delta (-x)}{\\delta x} + \\frac{\\delta 3xy}{\\delta x} + \\frac{\\delta 5xyz}{\\delta x}, \\frac{\\delta (-x)}{\\delta y} + \\frac{\\delta 3xy}{\\delta y} + \\frac{\\delta 5xyz}{\\delta y}, \\frac{\\delta (-x)}{\\delta z} + \\frac{\\delta 3xy}{\\delta z} + \\frac{\\delta 5xyz}{\\delta z}) $$\n",
    "$$ = (-1 + 3y + 5yz, 0 + 3x + 5xz, 0 + 0 + 5xy) = (-1 + 3y + 5yz, 3x + 5xz, 5xy) $$\n",
    "$$ \\nabla f (-1, 2, 1) = (-1 + 3 \\cdot 2 + 5 \\cdot 2 \\cdot 1, 3 \\cdot (-1) + 5 \\cdot (-1) \\cdot 1, 5 \\cdot (-1) \\cdot 2) = (15, -8, -10) $$"
   ]
  },
  {
   "cell_type": "markdown",
   "id": "b8a85a75",
   "metadata": {},
   "source": [
    "# Question 4\n",
    "Find the critical points (extreme points) for the following functions:\n",
    "\n",
    "$$f(x,y) = x^2 +y^2 −4x+6y+13$$\n",
    "\n",
    "$$ \\nabla f = (\\frac{\\delta f}{\\delta x}, \\frac{\\delta f}{\\delta y}) = (\\frac{\\delta (x^2 + y^2 - 4x + 6y + 13)}{\\delta x}, \\frac{\\delta (x^2 + y^2 - 4x + 6y + 13)}{\\delta y}) $$\n",
    "$$ = (\\frac{\\delta x^2}{\\delta x} + \\frac{\\delta y^2}{\\delta x} - \\frac{\\delta 4x}{\\delta x}+ \\frac{\\delta 6y}{\\delta x}+ \\frac{\\delta 13}{\\delta x}, \\frac{\\delta x^2}{\\delta y} + \\frac{\\delta y^2}{\\delta y} - \\frac{\\delta 4x}{\\delta y}+ \\frac{\\delta 6y}{\\delta y}+ \\frac{\\delta 13}{\\delta y})$$\n",
    "$$ = (2x + 0 - 4 + 0, 0 + 2y - 0 + 6 + 0) = (2x - 4, 2y + 6) $$\n",
    "$$ \\text{To find extreme points. Let } \\nabla f = 0 \\iff \\begin{cases}\n",
    "2x - 4 = 0 \\\\\n",
    "2y + 6 = 0\n",
    "\\end{cases} \n",
    "\\iff \\begin{cases}\n",
    "x = 2 \\\\\n",
    "y = -3\n",
    "\\end{cases} $$\n",
    "$$ \\text {Substitute (2, -3) to f: } f(2, -3) = 2^2 + (-3)^2 - 4 \\cdot 2 + 6 \\cdot (-3) + 13 = 36 $$\n",
    "\n",
    "$$f(x,y)=x^2 +2y^2 −2xy−2y+1$$\n",
    "\n",
    "$$f(x,y,z)=x^2 +y^2 +z^2 −2x+4y−6z$$\n",
    "\n",
    "$$f(x,y)=x^4 +y^4 −4xy$$"
   ]
  }
 ],
 "metadata": {
  "kernelspec": {
   "display_name": "Julia 1.12.1",
   "language": "julia",
   "name": "julia-1.12"
  },
  "language_info": {
   "file_extension": ".jl",
   "mimetype": "application/julia",
   "name": "julia",
   "version": "1.12.1"
  }
 },
 "nbformat": 4,
 "nbformat_minor": 5
}
